Add dead-code example with decision procedures

src/Language/PlutusIR.v
@@ -198,10 +198,29 @@ Arguments constructorName {_ _ _} _.
 (** * Named terms (all variables and binders are strings) *)
 Module NamedTerm.
 
-  Notation name := string.
-  Notation tyname := string.
-  Notation binderName := string.
-  Notation binderTyname := string.
+  Definition Unique (n : nat) := n.
+(*
+Inductive unique := Unique : nat -> unique.
+  Definition unique_dec : forall u u' : unique, {u = u'} + {u <> u'}.
+  Proof. decide equality. apply Nat.eq_dec. Defined.
+*)
+
+Definition Name (s : string) (n : nat) := string_of_nat n.
+(*
+Inductive name := Name : string -> unique -> name.
+
+Definition name_dec : forall n1 n2 : name, {n1 = n2} + {n1 <> n2}.
+Proof. decide equality. apply unique_dec. apply string_dec. Defined.
+*)
+
+Definition TyName (s : string) := s.
+
+Notation name := string (only parsing).
+Notation tyname := string (only parsing).
+Notation binderName := string (only parsing).
+Notation binderTyname := string (only parsing).
+
+
 
   (* These constructors should treat the type parameter
      as implicit too (this is already correctly generated for the recursive
