src/Language/PlutusIR/Transform/Compat.v
@@ -1,14 +1,25 @@
 Set Implicit Arguments.
 From PlutusCert Require Import Language.PlutusIR.
+From Coq Require Import
+  Bool.Bool
+  Utf8_core.
 Require Import Coq.Strings.String.
 Require Import Coq.Lists.List.
-From PlutusCert Require Import Util.List.
+From PlutusCert Require Import
+  Util.List
+  Analysis.Equality
+  .
 
 Generalizable All Variables.
 
+Import NamedTerm.
+
 Section Compatibility.
-  Import NamedTerm.
-  Variables (R : Term -> Term -> Type) (S : list Binding -> list Binding -> Type).
+    Context
+    (R : Term -> Term -> Type)
+    (dec_R : Term -> Term -> bool)
+  .
+
 
   Inductive Compat_Binding : Binding -> Binding -> Type :=
     | C_TermBind     : `{ R t t' -> Compat_Binding (TermBind s v t)
@@ -47,4 +58,137 @@ Section Compatibility.
     | C_Unwrap   : `{ R t t'                -> Compat (Unwrap t)
                                                     (Unwrap t')}
   .
+    Definition is_cong_binding  (b b' : Binding) : bool :=
+      match b, b' with
+        | (TermBind s v t), (TermBind s' v' t') => Strictness_eqb s s' && VDecl_eqb v v' && dec_R t t'
+        | (TypeBind v T), (TypeBind v' T') => TVDecl_eqb v v'  && Ty_eqb T T'
+        | (DatatypeBind d), (DatatypeBind d') => DTDecl_eqb d d'
+        | _, _                               => false
+      end
+    .
+
+
+    Definition is_cong (t t' : Term) : bool :=
+      match t, t' with
+        | (Let r bs t), (Let r' bs' t')      => Recursivity_eqb r r' && forall2b is_cong_binding bs bs' && dec_R t t'
+        | (Var n), (Var n')                  => String.eqb n n'
+        | (TyAbs n k t), (TyAbs n' k' t')    => String.eqb n n' && Kind_eqb k k' && dec_R t t'
+        | (LamAbs n T t), (LamAbs n' T' t')  => String.eqb n n'&& Ty_eqb T T' && dec_R t t'
+        | (Apply s t), (Apply s' t')         => dec_R s s' && dec_R t t'
+        | (Constant v), (Constant v')        => some_valueOf_eqb v v'
+        | (Builtin f), (Builtin f')          => func_eqb f f'
+        | (TyInst t T), (TyInst t' T')       => Ty_eqb T T' && dec_R t t'
+        | (Error T), (Error T')              => Ty_eqb T T'
+        | (IWrap T1 T2 t), (IWrap T1' T2' t') => Ty_eqb T1 T1' && Ty_eqb T2 T2' && dec_R t t'
+        | (Unwrap t), (Unwrap t')            => dec_R t t'
+        | _, _                               => false
+      end
+      .
+
+    Ltac split_hypos :=
+      match goal with
+      | H : (?x && ?y)%bool = true |- _ => apply andb_true_iff in H; destruct H; split_hypos
+      | _ => idtac
+      end.
+
+    Create HintDb Hints_soundness.
+    Hint Resolve
+      string_eqb_eq
+      Recursivity_eqb_eq
+      Strictness_eqb_eq
+      Kind_eqb_eq
+      Ty_eqb_eq
+      some_valueOf_eqb_eq
+      func_eqb_eq
+      VDecl_eqb_eq
+      TVDecl_eqb_eq
+      DTDecl_eqb_eq
+    : Hints_soundness.
+
+
+
+    Lemma is_cong_Binding_Compat_Binding : ∀ b b',
+        (∀ t t', dec_R t t' = true -> R t t') ->
+        is_cong_binding b b' = true -> Compat_Binding b b'.
+    Proof with eauto with reflection.
+      intros b b' H_term_sound H_dec.
+      destruct b, b'.
+      all: simpl in H_dec; try discriminate H_dec.
+      all: split_hypos.
+      - assert (s = s0)...
+        assert (v = v0)...
+        subst.
+        apply C_TermBind...
+      - assert (t = t1)...
+        assert (t0 = t2)...
+        subst.
+        apply C_TypeBind.
+      - assert (d = d0)...
+        subst.
+        apply C_DatatypeBind.
+    Qed.
+
+    Lemma is_cong_Bindings_Compat_Bindings : ∀ bs bs',
+        (∀ t t', dec_R t t' = true -> R t t') ->
+        forall2b is_cong_binding bs bs' = true -> Compat_Bindings bs bs'.
+    Proof with eauto.
+      intros bs.
+      induction bs.
+      all: intros bs' H_term_sound H_dec.
+      all: destruct bs'.
+      all: simpl in H_dec.
+      all: try discriminate H_dec.
+      - apply Compat_Bindings_Nil.
+      - split_hypos.
+        apply Compat_Bindings_Cons.
+        + apply is_cong_Binding_Compat_Binding...
+        + eauto.
+    Qed.
+
+    Lemma is_cong_Compat t t' :
+      (∀ t t', dec_R t t' = true -> R t t') ->
+      is_cong t t' = true -> Compat t t'.
+    Proof with eauto with reflection.
+      generalize t'.
+      clear t'.
+      intros t'.
+      induction t.
+      all: intros H_sound_R H_dec.
+      all: destruct t'.
+      all: simpl in H_dec.
+      all: try discriminate H_dec.
+      all: split_hypos.
+      - apply H_sound_R in H0.
+        apply Recursivity_eqb_eq in H.
+        subst.
+        eapply C_Let...
+        apply is_cong_Bindings_Compat_Bindings...
+      - apply String.eqb_eq in H_dec.
+        subst.
+        constructor.
+      - assert (b = s)...
+        assert (k = k0)...
+        subst.
+        eapply C_TyAbs...
+      - assert (b = s)...
+        assert (t = t1)...
+        subst.
+        apply C_LamAbs...
+      - apply C_Apply...
+      - assert (s = s0)...
+        subst.
+        apply C_Constant.
+      - assert (d = d0)... subst.
+        apply C_Builtin.
+      - assert (t0 = t1)... subst.
+        apply C_TyInst...
+      - assert (t = t0)... subst.
+        apply C_Error.
+      - assert (t = t2)...
+        assert (t0 = t3)...
+        subst.
+        apply C_IWrap...
+      - apply C_Unwrap...
+    Qed.
+
 End Compatibility.
