examples/timelock/DeadCode.v
@@ -1,0 +1,17 @@
+From Coq Require Import
+  Strings.String.
+From PlutusCert Require Import
+  PlutusIR
+  DeadCode
+  DeadCode.Decide.
+From Timelock Require Import
+  PreTerm
+  PostTerm.
+
+Open Scope string_scope.
+
+(*
+Eval cbv in t_pre.
+Eval cbv in t_post.
+*)
+Eval cbv in dec_Term t_pre t_post.
