src/Language/PlutusIR/Analysis/Equality.v
@@ -1,0 +1,536 @@
+Require Import Coq.Strings.String.
+Require Import Coq.Arith.PeanoNat.
+Require Import Coq.ZArith.BinInt.
+Require Import Coq.Bool.BoolEq.
+Require Import Coq.Lists.List.
+Require Import Ascii.
+Require Import Eqdep.
+Set Implicit Arguments.
+
+From PlutusCert Require Import Language.PlutusIR.
+Import NamedTerm.
+
+Definition EqDec := fun A : Type => forall x y : A, {x = y} + {x <> y}.
+
+
+Create HintDb Eqs.
+#[export] Hint Resolve Nat.eq_dec Z.eq_dec ascii_dec bool_dec string_dec list_eq_dec : Eqs.
+
+Ltac solveEq :=
+  intros;
+  unfold EqDec;
+  decide equality; auto with Eqs. (* debug auto with Eqs.*)
+
+Definition unit_dec: EqDec unit. Proof. solveEq. Defined.
+  #[export] Hint Resolve unit_dec : Eqs.
+
+Definition Strictness_dec: EqDec Strictness. solveEq. Defined.
+  #[export] Hint Resolve Strictness_dec : Eqs.
+
+  Definition Recursivity_dec : EqDec Recursivity. Proof. solveEq. Defined.
+  #[export] Hint Resolve Recursivity_dec : Eqs.
+
+Definition func_dec : EqDec DefaultFun. Proof. solveEq. Defined.
+  #[export] Hint Resolve func_dec: Eqs.
+
+Definition DefaultUni_dec : EqDec DefaultUni. solveEq. Defined.
+  #[export] Hint Resolve DefaultUni_dec : Eqs.
+
+Definition uniType_dec : forall t, EqDec (uniType t). intro t. destruct t; simpl; solveEq; solveEq. Defined.
+  #[export] Hint Resolve uniType_dec : Eqs.
+
+Definition valueOf_dec : forall t, EqDec (valueOf t). solveEq. apply uniType_dec. Defined.
+  #[export] Hint Resolve valueOf_dec : Eqs.
+
+Definition typeIn_dec : forall t, EqDec (typeIn t). solveEq. Defined.
+  #[export] Hint Resolve typeIn_dec : Eqs.
+
+(* Somewhat cumbersome, cannot use "decide equality" tactic *)
+Definition some_valueOf_dec: forall (x y : @some valueOf), {x = y} + {x <> y}.
+Proof.
+  intros x y.
+  refine (
+    match x, y with | @Some _ u  v, @Some _ u' v' =>
+    match DefaultUni_dec u u' with
+    | left eq   => _
+    | right neq => _
+    end end
+  ).
+  - subst. destruct (valueOf_dec v v').
+    + apply left. congruence.
+    + apply right. intros H.
+      inversion H .
+      inversion_sigma.
+      unfold eq_rect in H2.
+      assert (H3 : H0 = eq_refl). { apply UIP_refl. } (* I need UIP to reduce eq_rect and finish the proof, can this be done without? *)
+      rewrite H3 in H2.
+      contradiction.
+  - apply right. intros H.
+    inversion H. contradiction.
+Defined.
+  #[export] Hint Resolve some_valueOf_dec : Eqs.
+
+(* Somewhat cumbersome, cannot use "decide equality" tactic *)
+Definition some_typeIn_dec: forall (x y : @some typeIn), {x = y} + {x <> y}.
+Proof.
+  intros x y.
+  refine (
+    match x, y with | @Some _ u  v, @Some _ u' v' =>
+    match DefaultUni_dec u u' with
+    | left eq   => _
+    | right neq => _
+    end end
+  ).
+  - subst. destruct (typeIn_dec v v').
+    + apply left. congruence.
+    + apply right. intros H.
+      inversion H .
+      inversion_sigma.
+      unfold eq_rect in H2.
+      assert (H3 : H0 = eq_refl). { apply UIP_refl. } (* I need UIP to reduce eq_rect and finish the proof, can this be done without? *)
+      rewrite H3 in H2.
+      contradiction.
+  - apply right. intros H.
+    inversion H. contradiction.
+Defined.
+  #[export] Hint Resolve some_typeIn_dec : Eqs.
+
+Definition Kind_dec : EqDec Kind. solveEq. Defined.
+  #[export] Hint Resolve Kind_dec : Eqs.
+
+Definition Ty_dec: EqDec Ty. solveEq. Defined.
+  #[export] Hint Resolve Ty_dec : Eqs.
+
+Definition VDecl_dec: EqDec VDecl. Proof. solveEq. Defined.
+  #[export] Hint Resolve VDecl_dec : Eqs.
+
+Definition TVDecl_dec : EqDec TVDecl. Proof. solveEq. Defined.
+  #[export] Hint Resolve TVDecl_dec : Eqs.
+
+Definition constructor_dec : EqDec constructor. Proof. solveEq. Defined.
+  #[export] Hint Resolve constructor_dec : Eqs.
+
+Definition DTDecl_dec: EqDec DTDecl. Proof. solveEq. Defined.
+  #[export] Hint Resolve DTDecl_dec : Eqs.
+
+Lemma Term_dec : forall (x y : Term), {x = y} + {x <> y}
+  with binding_dec: forall (x y : Binding), {x = y} + {x <> y}.
+Proof.
+  - solveEq.
+  - solveEq.
+Defined.
+
+Definition pass_dec {name : Set} (name_dec : EqDec name) (p1 p2 : pass name) :
+  {p1 = p2} + {p1 <> p2}.
+  Proof. solveEq. Defined.
+
+Definition pair_dec {a b} (a_dec : EqDec a) (b_dec : EqDec b) : EqDec (a * b).
+  Proof. solveEq. Defined.
+(* boolean equality
+I define this separately from the dec_* functions to avoid carrying around
+proof terms at run-time.
+*)
+
+(*
+  TODO: do this cleanly with HasEqb/HasEqBool/HasEq
+  https://coq.inria.fr/library/Coq.Structures.Equalities.html
+*)
+
+Create HintDb reflection.
+
+(*
+  Note [#[export] Hints and name-collision]
+  ~~~~~~~~~~~~~~~~
+
+  When adding Nat.eqb_eq to a hint database using "#[export] Hint Resolve ->", Coq
+  generates a definition eqb_eq_l2r (note: not qualified by module name
+  anymore). The same happens when adding String.eqb_eq, thus causing a naming
+  conflict.
+  Current work-around is to alias the imported functions.
+*)
+(* Note [#[export] Hints and name-collision] *)
+Definition Z_eqb_eq := Z.eqb_eq.
+Definition nat_eqb_eq := Nat.eqb_eq.
+Definition string_eqb_eq := String.eqb_eq.
+#[export] Hint Resolve ->
+  andb_true_iff
+  nat_eqb_eq
+  Z_eqb_eq
+  string_eqb_eq
+  Ascii.eqb_eq
+  Bool.eqb_true_iff
+: reflection.
+
+#[export] Hint Resolve <-
+  andb_true_iff
+  nat_eqb_eq
+  Z_eqb_eq
+  string_eqb_eq
+  Ascii.eqb_eq
+  Bool.eqb_true_iff
+: reflection.
+Definition andb_and : forall s t, s && t = true -> s = true /\ t = true.
+Proof. auto with reflection. Qed.
+
+Ltac rewrite_eqbs := repeat (
+  match goal with
+  | Hyp : _ |- _ => apply andb_and in Hyp
+  end).
+
+(* Destruct all /\ hypotheses*)
+Ltac destruct_ands := repeat (
+  match goal with
+  | Hyp : ?l /\ ?r |- _ => destruct Hyp
+  end).
+
+Ltac bool_assumptions :=
+  repeat (rewrite_eqbs; destruct_ands).
+
+Ltac eqb_eq_tac :=
+  intros x y;
+  constructor; (* <-> *)
+
+  (* -> case*)
+  [ generalize y; clear y; induction x; intros y; (* get suitable IH *)
+    destruct y;
+    intros H;
+    repeat (rewrite_eqbs; destruct_ands); (* unfolds the call and rewrites && into /\*)
+    (f_equal || inversion H); (* Eliminate cases based on H, f_equal on same constructors*)
+    eauto with reflection
+
+  (* <- case *)
+  | intros H;
+    subst x;
+    induction y;
+    simpl;
+    eauto with reflection
+  ].
+
+
+Definition Eqb x := x -> x -> bool.
+Definition Eqb_eq := fun {a} (eqb : Eqb a) => forall (x y : a),
+  eqb x y = true <-> x = y.
+
+Definition unit_eqb: Eqb unit := fun x y => match x, y with
+  | tt, tt => true
+  end.
+Definition unit_eqb_eq : Eqb_eq unit_eqb.
+   Proof. eqb_eq_tac. Defined.
+
+#[export] Hint Resolve -> unit_eqb_eq : reflection.
+#[export] Hint Resolve <- unit_eqb_eq : reflection.
+
+
+Definition Strictness_eqb: Eqb Strictness := fun x y =>
+  match x, y with
+  | NonStrict, NonStrict => true
+  | Strict   , Strict    => true
+  | _, _                 => false
+  end.
+
+Definition Strictness_eqb_eq : Eqb_eq Strictness_eqb.
+Proof. eqb_eq_tac. Defined.
+#[export] Hint Resolve -> Strictness_eqb_eq : reflection.
+#[export] Hint Resolve <- Strictness_eqb_eq : reflection.
+
+Definition Recursivity_eqb : Eqb Recursivity := fun x y => match x, y with
+  | NonRec, NonRec => true
+  | Rec, Rec => true
+  | _, _ => false
+  end.
+
+Definition Recursivity_eqb_eq : Eqb_eq Recursivity_eqb.
+Proof. eqb_eq_tac. Qed.
+#[export] Hint Resolve -> Recursivity_eqb_eq : reflection.
+#[export] Hint Resolve <- Recursivity_eqb_eq : reflection.
+
+Definition func_eqb : Eqb DefaultFun := fun x y => match x, y with
+  | AddInteger , AddInteger => true
+  | SubtractInteger , SubtractInteger => true
+  | MultiplyInteger , MultiplyInteger => true
+  | DivideInteger , DivideInteger => true
+  | QuotientInteger , QuotientInteger => true
+  | RemainderInteger , RemainderInteger => true
+  | ModInteger , ModInteger => true
+  | LessThanInteger , LessThanInteger => true
+  | LessThanEqInteger , LessThanEqInteger => true
+  | GreaterThanInteger , GreaterThanInteger => true
+  | GreaterThanEqInteger , GreaterThanEqInteger => true
+  | EqInteger , EqInteger => true
+  | Concatenate , Concatenate => true
+  | TakeByteString , TakeByteString => true
+  | DropByteString , DropByteString => true
+  | SHA2 , SHA2 => true
+  | SHA3 , SHA3 => true
+  | VerifySignature , VerifySignature => true
+  | EqByteString , EqByteString => true
+  | LtByteString , LtByteString => true
+  | GtByteString , GtByteString => true
+  | IfThenElse , IfThenElse => true
+  | CharToString , CharToString => true
+  | Append , Append => true
+  | Trace , Trace => true
+  | _, _ => false
+  end.
+
+Definition func_eqb_eq : Eqb_eq func_eqb.
+Proof. eqb_eq_tac. Qed.
+#[export] Hint Resolve -> func_eqb_eq : reflection.
+#[export] Hint Resolve <- func_eqb_eq : reflection.
+
+Definition DefaultUni_eqb : Eqb DefaultUni := fun x y => match x, y with
+  | DefaultUniInteger , DefaultUniInteger => true
+  | DefaultUniByteString , DefaultUniByteString => true
+  | DefaultUniString , DefaultUniString => true
+  | DefaultUniChar , DefaultUniChar => true
+  | DefaultUniUnit , DefaultUniUnit => true
+  | DefaultUniBool , DefaultUniBool => true
+  | _, _ => false
+  end.
+
+Definition DefaultUni_eqb_eq : Eqb_eq DefaultUni_eqb.
+Proof. eqb_eq_tac. Qed.
+#[export] Hint Resolve -> DefaultUni_eqb_eq : reflection.
+#[export] Hint Resolve <- DefaultUni_eqb_eq : reflection.
+
+Definition uniType_eqb : forall t, Eqb (uniType t) := fun ty =>
+  match ty return Eqb (uniType ty) with
+  | DefaultUniInteger => Z.eqb
+  | DefaultUniChar    => Strings.Ascii.eqb
+  | DefaultUniUnit    => unit_eqb
+  | DefaultUniBool    => Bool.eqb
+  | DefaultUniByteString => String.eqb
+  | DefaultUniString    => String.eqb
+  end.
+
+Definition uniType_eqb_eq : forall t, Eqb_eq (uniType_eqb t).
+Proof.
+  intro t.
+  destruct t;
+  unfold Eqb_eq;
+  auto using Z.eqb_eq, string_eqb_eq, unit_eqb_eq, Ascii.eqb_eq, Nat.eqb_eq, Bool.eqb_true_iff.
+Qed.
+
+#[export] Hint Resolve -> uniType_eqb_eq : reflection.
+#[export] Hint Resolve <- uniType_eqb_eq : reflection.
+
+Definition valueOf_eqb : forall t, Eqb (valueOf t) := fun ty x y => match x, y with
+  | ValueOf _ x, ValueOf _ y => uniType_eqb ty x y
+  end.
+
+Definition valueOf_eqb_eq : forall t, Eqb_eq (@valueOf_eqb t).
+Proof.
+  intros t.
+  destruct t;
+  eqb_eq_tac.
+Qed.
+#[export] Hint Resolve -> valueOf_eqb_eq : reflection.
+#[export] Hint Resolve <- valueOf_eqb_eq : reflection.
+
+Definition some_valueOf_eqb: Eqb (@some valueOf) := fun x y => match x, y with
+  | @Some _ t v, @Some _ t' v' =>
+    match DefaultUni_dec t t' with
+    | left H => valueOf_eqb (eq_rect _ valueOf v _ H) v'
+    | _      => false
+    end
+  end.
+
+Definition some_valueOf_eqb_eq : Eqb_eq (some_valueOf_eqb).
+Proof.
+  eqb_eq_tac.
+  - destruct u, u0;
+    simpl in *;
+    f_equal;
+    inversion H;
+    auto with reflection.
+  - destruct u;
+    simpl;
+    destruct f; simpl;
+    auto with reflection.
+Qed.
+#[export] Hint Resolve -> some_valueOf_eqb_eq : reflection.
+#[export] Hint Resolve <- some_valueOf_eqb_eq : reflection.
+
+Definition typeIn_eqb : forall t, Eqb (typeIn t) := fun ty x y => match x, y with
+  | @TypeIn _, TypeIn _ => true
+  end.
+
+Definition typeIn_eqb_eq : forall t, Eqb_eq (@typeIn_eqb t).
+Proof.
+  intros t.
+  destruct t;
+  eqb_eq_tac.
+Qed.
+#[export] Hint Resolve -> typeIn_eqb_eq : reflection.
+#[export] Hint Resolve <- typeIn_eqb_eq : reflection.
+
+Definition some_typeIn_eqb : Eqb (@some typeIn) := fun x y => match x, y with
+  | @Some _ t v, @Some _ t' v' =>
+    match DefaultUni_dec t t' with
+    | left H => typeIn_eqb (eq_rect _ typeIn v _ H) v'
+    | _      => false
+    end
+  end.
+
+Definition some_typeIn_eqb_eq : Eqb_eq (some_typeIn_eqb).
+Proof.
+  eqb_eq_tac.
+  - destruct u, u0;
+    simpl in *;
+    f_equal;
+    inversion H;
+    auto with reflection.
+  - destruct u;
+    simpl;
+    destruct f; simpl;
+    auto with reflection.
+Qed.
+#[export] Hint Resolve -> some_typeIn_eqb_eq : reflection.
+#[export] Hint Resolve <- some_typeIn_eqb_eq : reflection.
+
+Fixpoint Kind_eqb (x y : Kind) : bool := match x, y with
+  | Kind_Base, Kind_Base => true
+  | Kind_Arrow K1 K2, Kind_Arrow K3 K4 => Kind_eqb K1 K3 && Kind_eqb K2 K4
+  | _, _ => false
+  end.
+
+Definition Kind_eqb_eq : Eqb_eq Kind_eqb.
+Proof. eqb_eq_tac. Defined.
+
+#[export] Hint Resolve -> Kind_eqb_eq : reflection.
+#[export] Hint Resolve <- Kind_eqb_eq : reflection.
+
+(* TODO: This is not correct yet. Because we have computation in types, we can not merely rely
+  on syntactic equality checking. *)
+Fixpoint Ty_eqb (x y : Ty) : bool := match x, y with
+  | Ty_Var X, Ty_Var Y => String.eqb X Y
+  | Ty_Fun T1 T2, Ty_Fun T3 T4 => Ty_eqb T1 T3 && Ty_eqb T2 T4
+  | Ty_IFix T1 U1, Ty_IFix T2 U2 => Ty_eqb T1 T2 && Ty_eqb U1 U2
+  | Ty_Forall X1 K1 T1, Ty_Forall X2 K2 T2 => String.eqb X1 X2 && Kind_eqb K1 K2 && Ty_eqb T1 T2
+  | Ty_Builtin s1, Ty_Builtin s2 => some_typeIn_eqb s1 s2
+  | Ty_Lam X1 K1 T1, Ty_Lam X2 K2 T2 => String.eqb X1 X2 && Kind_eqb K1 K2 && Ty_eqb T1 T2
+  | Ty_App S1 T1, Ty_App S2 T2 => Ty_eqb S1 S2 && Ty_eqb T1 T2
+  | _, _ => false
+  end.
+
+Definition Ty_eqb_eq : Eqb_eq Ty_eqb.
+Proof. Local Open Scope string_scope. eqb_eq_tac; try (inversion H).
+  - assert (b =? b = true) by eauto with reflection.
+    assert (Kind_eqb k k = true) by eauto with reflection.
+    rewrite H. rewrite H0. rewrite IHy. auto.
+  - assert (b =? b = true) by eauto with reflection.
+    assert (Kind_eqb k k = true) by eauto with reflection.
+    rewrite H. rewrite H0. rewrite IHy. auto.
+Defined.
+#[export] Hint Resolve -> Ty_eqb_eq : reflection.
+#[export] Hint Resolve <- Ty_eqb_eq : reflection.
+
+
+Definition TVDecl_eqb : Eqb TVDecl := fun x y => match x, y with
+  | TyVarDecl ty k, TyVarDecl ty' k' => String.eqb ty ty' && Kind_eqb k k'
+  end.
+
+Definition TVDecl_eqb_eq : Eqb_eq TVDecl_eqb.
+Proof. eqb_eq_tac. Defined.
+#[export] Hint Resolve -> TVDecl_eqb_eq : reflection.
+#[export] Hint Resolve <- TVDecl_eqb_eq : reflection.
+
+
+Definition VDecl_eqb: Eqb VDecl := fun x y => match x, y with
+  | VarDecl x ty, VarDecl x' ty' => String.eqb x x' && Ty_eqb ty ty'
+  end.
+Definition VDecl_eqb_eq : Eqb_eq VDecl_eqb.
+Proof. eqb_eq_tac. Defined.
+
+#[export] Hint Resolve -> VDecl_eqb_eq : reflection.
+#[export] Hint Resolve <- VDecl_eqb_eq : reflection.
+(* reminder: String.eqb_eq is opaque, perhaps this will be an
+issue later on*)
+
+
+
+Definition constructor_eqb : Eqb constructor := fun x y => match x, y with
+  | Constructor c n, Constructor c' n' => VDecl_eqb c c' && Nat.eqb n n'
+  end.
+
+Definition constructor_eqb_eq : Eqb_eq constructor_eqb.
+Proof. eqb_eq_tac. Qed.
+#[export] Hint Resolve -> constructor_eqb_eq : reflection.
+#[export] Hint Resolve <- constructor_eqb_eq : reflection.
+
+Definition list_eqb a (eqb : Eqb a) : Eqb (list a) := fix f xs ys :=
+  match xs, ys with
+  | nil, nil             => true
+  | cons x xs, cons y ys => eqb x y && f xs ys
+  | _, _                 => false
+  end.
+
+Definition list_eqb_eq a (a_eqb : Eqb a) (a_eqb_eq : Eqb_eq a_eqb) : Eqb_eq (list_eqb a_eqb).
+Proof.
+  eqb_eq_tac.
+  (* -> case for:  (x : a) = (y : a) *)
+  - apply a_eqb_eq; assumption.
+  (* <- case for: a_eqb ... && list_eqb ... = true *)
+  - unfold Eqb, Eqb_eq in *.
+    apply andb_true_iff_proj_r2l.
+    constructor.
+    + apply a_eqb_eq.
+      reflexivity.
+    + assumption.
+Qed.
+
+#[export] Hint Resolve -> list_eqb_eq : reflection.
+#[export] Hint Resolve <- list_eqb_eq : reflection.
+
+Definition DTDecl_eqb: Eqb DTDecl := fun x y => match x, y with
+  | Datatype tvd tvds n cs, Datatype tvd' tvds' n' cs' =>
+    TVDecl_eqb tvd tvd' && list_eqb TVDecl_eqb tvds tvds'
+      && String.eqb n n' && list_eqb constructor_eqb cs cs'
+    end.
+Definition DTDecl_eqb_eq : Eqb_eq DTDecl_eqb.
+
+Proof.
+  eqb_eq_tac.
+  - apply (list_eqb_eq TVDecl_eqb_eq).
+    assumption.
+  - apply (list_eqb_eq constructor_eqb_eq).
+    assumption.
+  - repeat (apply andb_true_iff_proj_r2l; constructor);
+     auto with reflection.
+    + apply (list_eqb_eq TVDecl_eqb_eq).
+      reflexivity.
+    + apply (list_eqb_eq constructor_eqb_eq).
+      reflexivity.
+Qed.
+#[export] Hint Resolve -> DTDecl_eqb_eq : reflection.
+#[export] Hint Resolve <- DTDecl_eqb_eq : reflection.
+
+
+
+
+
+
+
+Fixpoint Term_eqb (x y : Term) {struct x} : bool := match x, y with
+  | Let rec bs t, Let rec' bs' t' => Recursivity_eqb rec rec'
+      && list_eqb Binding_eqb bs bs'
+        && Term_eqb t t'
+  | Var n, Var n' => String.eqb n n'
+  | TyAbs n k t, TyAbs n' k' t' => String.eqb n n' && Kind_eqb k k' && Term_eqb t t'
+  | LamAbs n ty t, LamAbs n' ty' t' => String.eqb n n' && Ty_eqb ty ty' && Term_eqb t t'
+  | Apply s t, Apply s' t' => Term_eqb s s' && Term_eqb t t'
+  | Constant c, Constant c' => some_valueOf_eqb c c'
+  | Builtin f, Builtin f' => func_eqb f f'
+  | TyInst t ty, TyInst t' ty' => Term_eqb t t' && Ty_eqb ty ty'
+  | Error ty , Error ty' => Ty_eqb ty ty'
+  | IWrap ty1 ty2 t, IWrap ty1' ty2' t' => Ty_eqb ty1 ty1' && Ty_eqb ty2 ty2' && Term_eqb t t'
+  | Unwrap t, Unwrap t' => Term_eqb t t'
+  | _, _ => false
+  end
+with Binding_eqb (x y : Binding) {struct x} : bool := match x, y with
+  | TermBind s vd t, TermBind s' vd' t' => Strictness_eqb s s' && VDecl_eqb vd vd' && Term_eqb t t'
+  | TypeBind tvd ty, TypeBind tvd' ty' => TVDecl_eqb tvd tvd' && Ty_eqb ty ty'
+  | DatatypeBind  dtd, DatatypeBind dtd' => DTDecl_eqb dtd dtd'
+  | _, _ => false
+  end
+  .
