src/Language/PlutusIR/Analysis/Value.v
@@ -1,0 +1,157 @@
+From Coq Require Import
+  Strings.String
+  Lists.List
+  Bool.Bool
+  Arith.PeanoNat
+.
+
+From PlutusCert Require Import
+  Language.PlutusIR
+  Util.List
+  .
+
+Import NamedTerm.
+Import PeanoNat.Nat.
+
+(** ** Arity of built-in functions *)
+Definition arity (df : DefaultFun) : nat :=
+  match df with
+  | AddInteger => 2
+  | SubtractInteger => 2
+  | MultiplyInteger => 2
+  | DivideInteger => 2
+  | QuotientInteger => 2
+  | RemainderInteger => 2
+  | ModInteger => 2
+  | LessThanInteger => 2
+  | LessThanEqInteger => 2
+  | GreaterThanInteger => 2
+  | GreaterThanEqInteger => 2
+  | EqInteger => 2
+  | Concatenate => 2
+  | TakeByteString => 2
+  | DropByteString => 2
+  | SHA2 => 1
+  | SHA3 => 1
+  | VerifySignature => 3
+  | EqByteString => 2
+  | LtByteString => 2
+  | GtByteString => 2
+  | IfThenElse => 4
+  | CharToString => 1
+  | Append => 2
+  | Trace => 1
+  end.
+
+
+
+Inductive is_error : Term -> Prop :=
+  | IsError : forall T,
+      is_error (Error T).
+
+Inductive value : Term -> Prop :=
+  | V_LamAbs : forall x T t0,
+      value (LamAbs x T t0) 
+  | V_TyAbs : forall X K t,
+      value (TyAbs X K t)
+  | V_IWrap : forall F T v,
+      value v ->
+      ~ is_error v ->
+      value (IWrap F T v)
+  | V_Constant : forall u,
+      value (Constant u)
+  | V_Error : forall T,
+      value (Error T)
+  (** Builtins *) 
+  | V_Neutral : forall nv,
+      neutral_value 0 nv ->
+      value nv
+  (** If-Then-Else constructs 
+
+      NOTE (2021-11-4): Removed separate treatment of if-then-else for the sake of simplicity.
+  *)
+  (* | V_If : 
+      value (Builtin IfThenElse)
+  | V_If1 : forall T,
+      value (TyInst (Builtin IfThenElse) T)
+  | V_If2 : forall T cond,
+      value (Apply (TyInst (Builtin IfThenElse) T) cond)
+  | V_If3 : forall T cond t,
+      value (Apply (Apply (TyInst (Builtin IfThenElse) T) cond) t) *)
+
+with neutral_value : nat -> Term -> Prop :=
+  | NV_Builtin : forall n f,
+      (* NOTE (2021-11-4): Removed separate treatment of if-then-else for the sake of simplicity. *)
+      (* f <> IfThenElse -> *)
+      n < arity f ->
+      neutral_value n (Builtin f)
+  | NV_Apply : forall n nv v,
+      value v ->
+      ~ is_error v ->
+      neutral_value (S n) nv ->
+      neutral_value n (Apply nv v)
+  | NV_TyInst : forall n nv T,
+      neutral_value (S n) nv ->
+      neutral_value n (TyInst nv T)
+  .
+
+#[export] Hint Constructors value : core.
+#[export] Hint Constructors neutral_value : core.
+
+Scheme value__ind := Minimality for value Sort Prop
+  with neutral_value__ind := Minimality for neutral_value Sort Prop.
+
+Combined Scheme value__multind from 
+  value__ind,
+  neutral_value__ind.
+
+Definition neutral (t : Term) := neutral_value 0 t.
+
+#[export] Hint Unfold neutral : core.
+Definition is_error_b (t : Term) :=
+  match t with
+    | Error T => true
+    | _       => false
+  end.
+
+Lemma is_error_is_error_b : forall t, is_error_b t = true -> is_error t.
+Proof.
+  intros t H.
+  destruct t; inversion H.
+  constructor.
+Qed.
+
+Fixpoint
+  is_value' (n : nat) (t : Term) {struct t} :=
+  match t with
+    | LamAbs x T t0 => true
+    | TyAbs X K t   => true
+    | IWrap F T v   => is_value' n v && negb (is_error_b v)
+    | Constant u    => true
+    | Error T       => true
+
+
+    (* Duplication for the termination checker *)
+    | Builtin f   => ltb n (arity f)
+    | Apply nv v  => is_value' n v && negb (is_error_b v) && is_value' (S n) nv
+    | TyInst nv T => is_value' (S n) nv
+    | _ => false
+  end
+  .
+
+Definition is_value := is_value' 0.
+
+Definition is_neutral_value (n : nat) (t : Term) :=
+  match t with
+    | Builtin f   => is_value' n t
+    | Apply nv v  => is_value' n t
+    | TyInst nv T => is_value' n t
+    | _           => false
+  end.
+
+Lemma is_value_value : forall t, is_value t = true -> value t.
+Admitted.
+
+Lemma is_neutral_value_neutral_value : forall n t, is_neutral_value n t = true -> neutral_value n t.
+Admitted.
+
