src/Language/PlutusIR/Transform/DeadCode/DecideSound.v
@@ -1,0 +1,281 @@
+From Coq Require Import
+  String
+  List
+  Bool
+  Program
+  Utf8_core
+.
+
+From PlutusCert Require Import
+  Language.PlutusIR
+  Util
+  Analysis.UniqueBinders
+  Analysis.Purity
+  Analysis.Equality
+  Transform.Compat
+  Transform.DeadCode
+  Transform.DeadCode.Decide
+.
+
+Import NamedTerm.
+Import ListNotations.
+
+Definition P_Term t := forall t', dec_Term t t' = true -> dead_syn t t'.
+Definition P_Binding b := forall b', dec_Binding dec_Term b b' = true -> dead_syn_binding b b'.
+
+Ltac split_hypos :=
+  match goal with
+  | H : (?x && ?y)%bool = true |- _ => apply andb_true_iff in H; destruct H; split_hypos
+  | _ => idtac
+  end.
+
+
+Lemma H_safely_removed bs bs':
+    forallb (fun b => safely_removed b (map name_Binding bs')) bs = true ->
+    ∀ b : Binding, In b bs → name_removed b bs' → pure_binding [] b.
+Proof with eauto with reflection.
+  intros H_dec.
+  intros b H_In H_removed.
+  unfold safely_removed in H_dec.
+  rewrite forallb_forall in H_dec. (* why did rewrite accept a <-> ? was also possible with eapply -> ..., but generated an existential for x *)
+  apply H_dec in H_In as H_dec_andb.
+  clear H_dec H_In.
+
+  destruct (negb
+    (existsb (String.eqb (name_Binding b))
+       (map name_Binding bs')))
+       eqn:H_1.
+  + apply is_pure_binding_pure_binding...
+
+  (* contradiction *)
+  + apply negb_false_iff in H_1.
+    unfold name_removed in *.
+    apply existsb_exists in H_1.
+    destruct H_1 as [x [H_in H_name_b_eq_x]].
+    apply String.eqb_eq in H_name_b_eq_x.
+    subst.
+    contradiction.
+Qed.
+
+Lemma H_find_binding' bs bs' :
+  (∀ b, In b bs -> P_Binding b) ->
+    forallb (fun b' => find_Binding dec_Term b' bs) bs' = true ->
+    ∀ b', In b' bs' ->
+       ∃ x, In x bs /\
+         name_Binding x = name_Binding b' /\
+         dead_syn_binding x b'
+    .
+Proof with eauto with reflection.
+  intro H_P_Binding.
+  rewrite forallb_forall.
+  intros H_dec b' H_In.
+  apply H_dec in H_In as H_find_b'.
+  clear H_dec.
+  induction bs as [ | b ].
+  - discriminate H_find_b'.
+  - simpl in H_find_b'.
+    destruct (name_Binding b =? name_Binding b')%string
+      eqn:H_name_eq.
+
+    (* b related to b' *)
+    + exists b.
+      repeat split...
+      * constructor...
+      * assert (H : P_Binding b).
+        ++ apply H_P_Binding.
+           constructor...
+        ++ unfold P_Binding in H...
+
+
+    (* a not related to b' *)
+    + apply IHbs in H_find_b' as H_ex. clear IHbs.
+      * destruct H_ex as [x [H_x_In [H_eq_name H_dead_syn]]].
+        assert (In x (b :: bs)). { apply in_cons... }
+        exists x...
+      * intros b0 H_b0_in.
+        apply H_P_Binding.
+        apply in_cons...
+Qed.
+
+Create HintDb Hints_bindings.
+#[local]
+Hint Resolve
+  H_safely_removed : Hints_bindings.
+#[local]
+Hint Constructors
+  dead_syn_bindings : Hints_bindings.
+#[local]
+Hint Resolve
+  H_safely_removed
+  H_find_binding' : Hints_bindings.
+#[local]
+Hint Constructors
+  dead_syn
+  dead_syn_binding
+  dead_syn_bindings
+  : reflection.
+
+Lemma dec_Bindings_sound' : ∀ bs bs',
+  (∀ b, In b bs -> P_Binding b) ->
+  dec_Bindings dec_Term bs bs' = true -> dead_syn_bindings bs bs'.
+Proof with eauto with Hints_bindings.
+  intros H_P_bs bs bs' H.
+  simpl in H.
+  unfold dec_Bindings in H.
+  split_hypos.
+  eapply dc_bindings...
+Qed.
+
+
+Lemma dec_TermBind_sound : ∀ s v t b b',
+  b = TermBind s v t ->
+  P_Term t -> 
+  dec_Binding dec_Term b b' = true ->
+  dead_syn_binding b b'.
+Proof with eauto with reflection.
+  intros s v t b b' H_eq H_P_Term H_dec.
+  unfold P_Term in *.
+  subst.
+  simpl in H_dec.
+  destruct b'.
+  all: try discriminate.
+  split_hypos.
+  assert (s = s0)...
+  assert (v = v0)...
+  subst...
+Qed.
+
+Lemma dec_TypeBind_sound : ∀ v ty b b',
+  b = TypeBind v ty ->
+  dec_Binding dec_Term b b' = true ->
+  dead_syn_binding b b'.
+Proof with eauto with reflection.
+  intros v ty b b' H_eq H_dec.
+  subst.
+  destruct b'.
+  all: try discriminate.
+  simpl in H_dec.
+  split_hypos.
+  assert (v = t)... subst.
+  assert (ty = t0)... subst...
+Qed.
+
+Lemma dec_DatatypeBind_sound : ∀ dtd b b',
+  b = DatatypeBind dtd ->
+  dec_Binding dec_Term b b' = true ->
+  dead_syn_binding b b'.
+Proof with eauto with reflection.
+  intros dtd b b' H_eq H_dec.
+  subst.
+  destruct b'.
+  all: try discriminate.
+  simpl in H_dec.
+  split_hypos.
+  assert (dtd = d)... subst...
+Qed.
+
+Lemma all_pure : ∀ bs,
+  forallb (is_pure_binding []) bs = true ->
+  Forall (pure_binding []) bs.
+Proof.
+  intros bs H_dec.
+  apply Forall_forall.
+  intros b H_In.
+  rewrite forallb_forall in H_dec.
+  auto using is_pure_binding_pure_binding.
+Qed.
+
+#[local]
+Hint Resolve all_pure : reflection.
+#[local]
+Hint Resolve dec_Bindings_sound' : reflection.
+#[local]
+Hint Resolve
+  dec_TermBind_sound 
+  dec_TypeBind_sound 
+  dec_DatatypeBind_sound 
+  : reflection.
+#[local]
+Hint Constructors Compat : reflection.
+
+Theorem dec_Term_Binding_sound :
+  (∀ t, P_Term t) /\ (∀ b, P_Binding b).
+Proof with eauto with reflection.
+  apply Term__multind with (P := P_Term) (Q := P_Binding).
+  all: intros.
+
+  (* P_Term (Let rec bs t) *)
+  - unfold P_Term in *.
+    intros t' H_dec_Term.
+    simpl in H_dec_Term.
+    destruct t'; simpl in H_dec_Term.
+    all: split_hypos.
+    {
+      destruct (dec_Bindings dec_Term bs l) eqn:H_dec_bs.
+      all: split_hypos.
+      (* H_dec_Term: then branch *)
+      * split_hypos.
+
+        assert (H_bindings : dead_syn_bindings bs l).
+        {
+          apply ForallP_Forall in H.
+          rewrite -> Forall_forall in H...
+        }
+        assert (H_eq_rec : rec = r)... subst.
+        eapply dc_delete_bindings...
+
+      (* H_dec_Term: else branch *)
+      * eapply dc_delete_let...
+    }
+    all: try eapply dc_delete_let...
+
+  - unfold P_Term.
+    destruct t'.
+    all: intro H_dec; try discriminate H_dec.
+    assert (s = s0)... subst...
+  - unfold P_Term.
+    destruct t'.
+    all: intro H_dec; try discriminate H_dec.
+    simpl in H_dec. split_hypos.
+    assert (s = s0)... subst.
+    assert (k = k0)... subst...
+
+  - unfold P_Term; destruct t'; intro H_dec; try discriminate H_dec; simpl in H_dec; split_hypos.
+    assert (s = s0)...
+    assert (t = t1)... subst...
+  - unfold P_Term; destruct t'; intro H_dec; try discriminate H_dec; simpl in H_dec; split_hypos.
+    idtac...
+
+  - unfold P_Term; destruct t'; intro H_dec; try discriminate H_dec; simpl in H_dec; split_hypos.
+    assert (s = s0)... subst...
+
+  - unfold P_Term; destruct t'; intro H_dec; try discriminate H_dec; simpl in H_dec; split_hypos.
+    assert (d = d0)... subst...
+
+  - unfold P_Term; destruct t'; intro H_dec; try discriminate H_dec; simpl in H_dec; split_hypos.
+    assert (t0 = t1)... subst...
+
+  - unfold P_Term; destruct t'; intro H_dec; try discriminate H_dec; simpl in H_dec; split_hypos.
+    assert (t = t0)... subst...
+
+  - unfold P_Term; destruct t'; intro H_dec; try discriminate H_dec; simpl in H_dec; split_hypos.
+    assert (t = t2)... subst.
+    assert (t0 = t3)... subst...
+
+  - unfold P_Term; destruct t'; intro H_dec; try discriminate H_dec; simpl in H_dec; split_hypos.
+    idtac...
+
+  - unfold P_Binding...
+  - unfold P_Binding...
+  - unfold P_Binding...
+Qed.
+
+Corollary dec_Term_sound : ∀ t t', dec_Term t t' = true -> dead_syn t t'.
+Proof.
+  apply dec_Term_Binding_sound.
+Qed.
+
+Corollary dec_Binding_sound : ∀ t t', dec_Term t t' = true -> dead_syn t t'.
+Proof.
+  apply dec_Term_Binding_sound.
+Qed.
