src/Util.v
@@ -266,3 +266,25 @@ Definition zip_with {A B C} (f : A -> B -> C) : list A -> list B -> list C :=
 
 Notation " g ∘ f " := (compose g f)
   (at level 40, left associativity).
+
+From Coq Require Import Strings.String.
+Open Scope string_scope.
+
+Fixpoint string_of_nat_aux (time n : nat) (acc : string) : string :=
+  let d := match n mod 10 with
+           | 0 => "0" | 1 => "1" | 2 => "2" | 3 => "3" | 4 => "4" | 5 => "5"
+           | 6 => "6" | 7 => "7" | 8 => "8" | _ => "9"
+           end in
+  let acc' := d ++ acc in
+  match time with
+    | 0 => acc'
+    | S time' =>
+      match n / 10 with
+        | 0 => acc'
+        | n' => string_of_nat_aux time' n' acc'
+      end
+  end.
+Definition string_of_nat (n : nat) : string :=
+  string_of_nat_aux n n "".
+Close Scope string_scope.
+
